\begin{answer}
    Since we have $h(x) = g(\theta^T x)$, we have 
    $\partial h(x) / \partial \theta_j = h(x) (1 - h(x)) x_j$.

    Thus,
    $$
        \frac{\partial \log h_\theta(x^{(i)})}{\partial \theta_j} = (1 - h_\theta(x^{(i)})) x_j^{(i)}
    $$
    and
    $$
        \frac{\partial \log (1 - h_\theta(x^{(i)}))}{\partial \theta_j} = - h_\theta(x^{(i)}) x_j^{(i)}
    $$

    Thus, we have
    \begin{align*}
        \frac{\partial J(\theta)}{\partial \theta_j} &= - \frac{1}{n} \sum_{i = 1}^{n} y^{(i)} (1 - h_\theta(x^{(i)})) x_j^{(i)} - (1 - y^{(i)}) h_\theta(x^{(i)}) x_j^{(i)} \\
        &= - \frac{1}{n} \sum_{i = 1}^{n} (y^{(i)} - h_\theta(x^{(i)})) x_j^{(i)}
    \end{align*}

    Therefore, the (j, k)th entry of the Hessian is
    \begin{align*}
        H_{jk} &= \frac{\partial^2 J(\theta)}{\partial \theta_j \partial \theta_k} \\
        &= \frac{1}{n} \sum_{i = 1}^{n} h_\theta(x^{(i)}) (1 - h_\theta(x^{(i)})) x_j^{(i)} x_k^{(i)}
    \end{align*}

    Since $X = x x^T$ if and only if $X_{jk} = x_j x_k$, we have
    $$
        H = \frac{1}{n} \sum_{i = 1}^{n} h_\theta(x^{(i)}) (1 - h_\theta(x^{(i)})) x^{(i)} (x^{(i)})^T
    $$

    We need to show that $z^T H z \geq 0$ for any vector $z$.

    \begin{align*}
        z^T H z &= \frac{1}{n} \sum_{i = 1}^{n} z^T h_\theta(x^{(i)}) (1 - h_\theta(x^{(i)})) x^{(i)} (x^{(i)})^T z \\
        &= \frac{1}{n} \sum_{i = 1}^{n} h_\theta(x^{(i)}) (1 - h_\theta(x^{(i)})) ((x^{(i)})^T z) (z^T x^{(i)}) \\
        &= \frac{1}{n} \sum_{i = 1}^{n} h_\theta(x^{(i)}) (1 - h_\theta(x^{(i)})) ((x^{(i)})^T z)^2 \\
        &\geq 0
    \end{align*}
    At the last step, we used the fact that $h_\theta(x^{(i)}) \in [0, 1]$.
\end{answer}
