\begin{answer}
    Since we have
    \begin{align*}
        p(y=1|x;\phi,\mu_0,\mu_1,\Sigma) &= \frac{p(y=1) p(x|y=1)}{p(y=0) p(x|y=0) + p(y=1)p(x|y=1)} \\
        &= \frac{1}{1 + \frac{p(y=0)p(x|y=0)}{p(y=1)p(x|y=1)}} 
    \end{align*}
    We just need to show that the term in the denominator is equal to
    the exponential term in the problem description.
    Put in the equations for $p(x|y=0)$ and $p(x|y=1)$, we have
    \begin{align*}
        \frac{p(y=0)p(x|y=0)}{p(y=1)p(x|y=1)} &= \frac{(1-\phi) \frac{1}{(2\pi)^{n/2}|\Sigma|^{1/2}} \exp\left(-\frac{1}{2}(x-\mu_0)^T\Sigma^{-1}(x-\mu_0)\right)}{\phi \frac{1}{(2\pi)^{n/2}|\Sigma|^{1/2}} \exp\left(-\frac{1}{2}(x-\mu_1)^T\Sigma^{-1}(x-\mu_1)\right)} \\
        &= \frac{1-\phi}{\phi} \exp\left(-\frac{1}{2}(x-\mu_0)^T\Sigma^{-1}(x-\mu_0) + \frac{1}{2}(x-\mu_1)^T\Sigma^{-1}(x-\mu_1)\right)
    \end{align*}
    After rearranging the terms, and setting $\theta = - \Sigma^{-1}(\mu_1 - \mu_0)$, $\theta_0 = \frac{1}{2}(\mu_0^T\Sigma^{-1}\mu_0 - \mu_1^T\Sigma^{-1}\mu_1) - \log\frac{1-\phi}{\phi}$, we have
    \begin{align*}
        \frac{p(y=0)p(x|y=0)}{p(y=1)p(x|y=1)} &= \exp(-(\theta^Tx + \theta_0))
    \end{align*}
    which is exactly the exponential term in the problem description.
\end{answer}
