\begin{answer}
    Expected value of $Y$ is
    $$
    \E(Y; \eta) = \int y p(y; \eta) dy = \int y b(y) \exp(\eta y - a(\eta)) dy
    $$
    Since we have:
    $$
    a(\eta) = \log \int b(y) \exp(\eta y) dy
    $$
    We can take the derivative of $a(\eta)$ with respect to $\eta$:
    $$
    \frac{\partial}{\partial \eta} a(\eta) = \frac{\int y b(y) \exp(\eta y) dy}{\int b(y) \exp(\eta y) dy} = \frac{\int y b(y) \exp(\eta y - a(\eta)) dy}{\int b(y) \exp(\eta y - a(\eta)) dy} = \E[Y; \eta]
    $$
    The last equality is due to the fact that the integral of probability density function is 1.
\end{answer}
