\begin{answer}
    \begin{align*}
        \arg\min_\theta \KL(\hat{P} \parallel P_\theta) &= \arg\min_\theta \sum_{x \in \mathcal{X}} \hat{P}(x) \log \frac{\hat{P}(x)}{P_\theta(x)} \\
        &= \arg\min_\theta \sum_{x \in \mathcal{X}} \hat{P}(x) \log \hat{P}(x) - \sum_{x \in \mathcal{X}} \hat{P}(x) \log P_\theta(x) \\
        &= \arg\min_\theta - \sum_{x \in \mathcal{X}} \hat{P}(x) \log P_\theta(x) \\
        &= \arg\min_\theta - \sum_{x \in \mathcal{X}} \hat{P}(x) \log \prod_{i=1}^n P_\theta(x^{(i)}) \\
        &= \arg\min_\theta - \sum_{x \in \mathcal{X}} \hat{P}(x) \sum_{i=1}^n \log P_\theta(x^{(i)}) \\
        &= \arg\min_\theta - \sum_{i=1}^n \sum_{x \in \mathcal{X}} \hat{P}(x) \log P_\theta(x^{(i)}) \\
        &= \arg\min_\theta - \sum_{i=1}^n \sum_{x \in \mathcal{X}} 1\{\xsi=x\} \log P_\theta(x^{(i)}) \\
        &= \arg\min_\theta - \sum_{i=1}^n \log P_\theta(x^{(i)}) \\
        &= \arg\max_\theta \sum_{i=1}^n \log P_\theta(x^{(i)})
    \end{align*}
\end{answer}
